Hybrid/Completeness.lean
@@ -1,9 +1,8 @@
-import Hybrid.Truth
+import Hybrid.Soundness
 import Hybrid.ProofUtils
-import Hybrid.FormCountable
 
 section Lemmas
-  theorem satisfiable_iff_nocontradiction (Γ : Set Form) : Γ.satisfiable ↔ Γ ⊭ ⊥ := by
+  theorem satisfiable_iff_nocontradiction (Γ : Set (Form N)) : satisfiable Γ ↔ Γ ⊭ ⊥ := by
     apply Iff.intro <;> {
     . intro h
       simp at h ⊢
@@ -11,35 +10,33 @@ section Lemmas
       exact h
     }
   
-  theorem unsatisfiable_iff_contradiction (Γ : Set Form) : ¬Γ.satisfiable ↔ Γ ⊨ ⊥ := by
+  theorem unsatisfiable_iff_contradiction (Γ : Set (Form N)) : ¬satisfiable Γ ↔ Γ ⊨ ⊥ := by
     conv => rhs; rw [←@not_not (Γ ⊨ ⊥)]
     apply Iff.not
     apply satisfiable_iff_nocontradiction
   
-  theorem notsatnot {Γ : Set Form} {φ : Form} : (Γ⊨φ) ↔ ¬(Γ ∪ {∼φ}).satisfiable := by
+  theorem notsatnot {Γ : Set (Form N)} {φ : Form N} : (Γ⊨φ) ↔ ¬satisfiable (Γ ∪ {∼φ}) := by
     rw [unsatisfiable_iff_contradiction, ←SemanticDeduction, ←Form.neg, Entails, Entails]
     conv => rhs; intro M s g h; rw [neg_sat, neg_sat, not_not]
 
-  theorem notprove_consistentnot : (Γ ⊬ φ) ↔ (Γ ∪ {∼φ}).consistent := by
-    apply Iff.intro
-    . intro h
-      rw [←@not_not ((Γ ∪ {∼φ}).consistent)]
-      intro habs
-      rw [Set.consistent, not_not, ←Proof.Deduction, ←Form.neg, Proof.dn_equiv_premise] at habs
-      contradiction
-    . intro h
-      rw [Set.consistent, ←Proof.Deduction, ←Form.neg,  Proof.dn_equiv_premise] at h
-      exact h
+  theorem notprove_consistentnot : (Γ ⊬ φ) → consistent (Γ ∪ {∼φ}) := by
+    intro h
+    rw [←@not_not (consistent (Γ ∪ {∼φ}))]
+    intro habs
+    have ⟨habs, _⟩ := not_forall.mp habs
+    apply h
+    exact Proof.dn_equiv_premise.mp (Proof.Deduction.mpr habs)
+
 end Lemmas
 
 
-def completeness_statement := (∀ (Γ : Set Form) (φ : Form), Γ ⊨ φ → Γ ⊢ φ)
-def cons_sat_statement     := (∀ (Γ : Set Form), Γ.consistent → Γ.satisfiable)
+def completeness_statement := λ (N : Set ℕ) => (∀ (Γ : Set (Form N)) (φ : Form N), Γ ⊨ φ → (∃ _ : Γ ⊢ φ, True))
+def cons_sat_statement     := λ (N : Set ℕ) => (∀ (Γ : Set (Form N)), consistent Γ → satisfiable Γ)
 
-theorem ModelExistence : completeness_statement ↔ cons_sat_statement := by
+theorem ModelExistence {N : Set ℕ} : completeness_statement N ↔ cons_sat_statement N := by
   apply Iff.intro
   . intro h
-    rw [←@not_not (cons_sat_statement)]
+    rw [←@not_not (cons_sat_statement N)]
     intro habs
     rw [cons_sat_statement, negated_universal] at habs
     match habs with
@@ -47,17 +44,24 @@ theorem ModelExistence : completeness_statement ↔ cons_sat_statement := by
       rw [negated_impl] at hw
       have ⟨consistent, not_satisfiable⟩  := hw
       rw [unsatisfiable_iff_contradiction] at not_satisfiable
-      have by_completeness := (h Δ ⊥) not_satisfiable
-      contradiction
-  . rw [contraposition cons_sat_statement completeness_statement]
+      have ⟨by_completeness, _⟩ := (h Δ ⊥) not_satisfiable
+      exact consistent by_completeness
+  . rw [contraposition (cons_sat_statement N) (completeness_statement N)]
     intro h
-    simp only [completeness_statement, not_forall, negated_impl,
-            notprove_consistentnot, notsatnot, ←conj_comm] at h
+    simp only [completeness_statement, not_forall, negated_impl, notsatnot, ←conj_comm] at h
     simp only [cons_sat_statement, not_forall, negated_impl]
-    have ⟨Γ, φ, wit⟩ := h
+    have ⟨Γ, φ, wit_l, wit_r⟩ := h
     exists (Γ ∪ {∼φ})
+    apply And.intro
+    . apply notprove_consistentnot
+      intro pf
+      apply wit_r
+      exists pf
+    . assumption
 
-theorem Completeness : (∀ (Γ : Set Form) (φ : Form), Γ ⊨ φ → Γ ⊢ φ) := by
+theorem Completeness : (∀ (Γ : Set (Form N)) (φ : Form N), Γ ⊨ φ → Γ ⊢ φ) := by
+  intros h1 h2 h3; apply Exists.choose
+  revert h1 h2 h3
   rw [←completeness_statement, ModelExistence]
   unfold cons_sat_statement
   admit
