Hybrid/ExistenceLemma.lean
@@ -1,42 +1,40 @@
-import Hybrid.CompletedModel
 import Hybrid.Lindenbaum
 import Hybrid.ProofUtils
 
 open Proof
 
-def conjunction' (L : List Form) : Form :=
+def conjunction' (L : List (Form N)) : Form N :=
   match L with
     | []     => ⊥ ⟶ ⊥
     | [h]    => h
     | h :: t => h ⋀ conjunction' t
 
-def Set.has_wit_conj (Γ : Set Form) : Form → Form → Prop
-  | (ex x, ψ), φ => ∃ i : NOM, ◇(((ex x, ψ) ⟶ ψ[i//x]) ⋀ φ) ∈ Γ 
+def has_wit_conj (Γ : Set (Form N)) : Form N → Form N → Prop
+  | (ex x, ψ), φ => ∃ i : NOM N, ◇(((ex x, ψ) ⟶ ψ[i//x]) ⋀ φ) ∈ Γ 
   | _, _         => True
 
-lemma l313 {τ χ : Form} (h1 : is_substable χ y x) (h2 : occurs y τ = false) (h3 : occurs y χ = false) :
+lemma l313 {τ χ : Form N} (h1 : is_substable χ y x) (h2 : occurs y τ = false) (h3 : occurs y χ = false) :
   ⊢ (◇ τ ⟶ ex y, ◇(((ex x, χ) ⟶ χ[y//x]) ⋀ τ)) := by
   have l1 := Γ_empty.mpr (rename_bound_ex h3 h1)
   have l2 := Γ_empty.mp (Γ_conj_elim_l l1)
-  have l3 := @b361 (ex x, χ) y (χ[y//x])
+  have l3 := @b361 N y (χ[y//x]) (ex x, χ)
   have l4 := mp l3 l2
-  have l5 := tautology (@ax_1 ((ex y, (ex x, χ)⟶χ[y//x])) τ)
+  have l5 := tautology (@ax_1 N ((ex y, (ex x, χ)⟶χ[y//x])) τ)
   have l6 := mp l5 l4
-  have l7 := tautology (@imp_refl τ)
-  have l8 := tautology (@conj_intro_hs τ ((ex y, (ex x, χ)⟶χ[y//x])) τ)
+  have l7 := tautology (@imp_refl N τ)
+  have l8 := tautology (@conj_intro_hs N τ ((ex y, (ex x, χ)⟶χ[y//x])) τ)
   have l9 := mp (mp l8 l6) l7
-  have l10 := @b362' y τ ((ex x, χ)⟶χ[y//x]) (notoccurs_notfree h2)
+  have l10 := @b362' N y ((ex x, χ)⟶χ[y//x]) τ (notoccurs_notfree h2)
   have l11 := hs l9 l10
   have l12 := diw_impl l11
   have l13 := hs l12 ax_brcn_contrap
   exact l13
 
-lemma l313' {Δ : Set Form} (mcs : Δ.MCS) (wit : Δ.witnessed) (mem : ◇φ ∈ Δ) : ∀ ψ : Form, Δ.has_wit_conj ψ φ := by
+lemma l313' {Δ : Set (Form N)} (mcs : MCS Δ) (wit : witnessed Δ) (mem : ◇φ ∈ Δ) : ∀ ψ : Form N, has_wit_conj Δ ψ φ := by
   intro ψ
-  unfold Set.has_wit_conj
+  unfold has_wit_conj
   split
   . next _ _ x ψ =>
-      rw [←MCS_pf_iff mcs] at mem
       have ⟨y, geq, nocc, subst⟩ := (φ ⟶ ψ ⟶ all x, ⊥).new_var_properties
       have y_ne_x : y ≠ x := by
         intro habs
@@ -45,8 +43,7 @@ lemma l313' {Δ : Set Form} (mcs : Δ.MCS) (wit : Δ.witnessed) (mem : ◇φ ∈
       have subst := subst x
       simp [occurs, is_substable, is_free] at nocc subst
       have := Γ_theorem (l313 subst.2 nocc.1 nocc.2) Δ
-      have mem' := Γ_mp this mem
-      rw [MCS_pf_iff mcs] at mem'
+      have mem' := MCS_pf mcs (Γ_mp this (Γ_premise mem))
       have has_wit := wit mem'
       simp [subst_nom, y_ne_x] at has_wit ⊢
       admit
@@ -55,7 +52,7 @@ lemma l313' {Δ : Set Form} (mcs : Δ.MCS) (wit : Δ.witnessed) (mem : ◇φ ∈
 -- ◇ (((ex x, ψ)⟶ψ[y//x])⋀φ)
 -- ◇ ((ex x, ψ⟶ψ[i//x])⋀φ)
 
-def witness_conditionals (enum : ℕ → Form) (n : ℕ) {Δ : Set Form} (mcs : Δ.MCS) (wit : Δ.witnessed) (mem : ◇φ ∈ Δ) : ∃ (l : List Form), l ≠ [] ∧ ◇conjunction' l ∈ Δ :=
+def witness_conditionals (enum : ℕ → Form N) (n : ℕ) {Δ : Set (Form N)} (mcs : MCS Δ) (wit : witnessed Δ) (mem : ◇φ ∈ Δ) : ∃ (l : List (Form N)), l ≠ [] ∧ ◇conjunction' l ∈ Δ :=
   match n with
   | 0   => by exists [φ]; simp only [ne_eq, not_false_eq_true, conjunction', true_and, mem]
   | n+1 => by
@@ -68,23 +65,23 @@ def witness_conditionals (enum : ℕ → Form) (n : ℕ) {Δ : Set Form} (mcs : 
               exact ⟨((ex x, ψ_n) ⟶ ψ_n[i_n//x]) :: prev_l, by simp, by rw [conjunction']; exact curr_mem; exact prev_nnil⟩
            | _        => exact ⟨prev_l, prev_nnil, prev_mem⟩ 
 
-def succesor_set' (enum : ℕ → Form) {Δ : Set Form} (mcs : Δ.MCS) (wit : Δ.witnessed) (mem : ◇φ ∈ Δ) : Set Form :=
+def succesor_set' (enum : ℕ → Form N) {Δ : Set (Form N)} (mcs : MCS Δ) (wit : witnessed Δ) (mem : ◇φ ∈ Δ) : Set (Form N) :=
   {ψ | □ψ ∈ Δ} ∪ {φ | ∃ n : ℕ, φ ∈ (witness_conditionals enum n mcs wit mem).choose}
 
   
 
-
-def Set.has_wit_of (Γ : Set Form) : Form → Prop
+/-
+def Set.has_wit_of (Γ : Set (Form N)) : Form → Prop
   | ex x, φ => ∃ (i : NOM), (ex x, φ ⟶ φ[i//x]) ∈ Γ 
   | _       => True
 
-def Set.list_wit {Γ : Set Form} (enum : ℕ → Form) (n : ℕ) (h : ∀ i : ℕ, i < n → Γ.has_wit_of (enum i)) : List Form :=
+def Set.list_wit {Γ : Set (Form N)} (enum : ℕ → Form N) (n : ℕ) (h : ∀ i : ℕ, i < n → Γ.has_wit_of (enum i)) : List (Form N) :=
   match n with
   | 0   =>    []
   | n+1 =>    sorry
 
-theorem set_family (enum : ℕ → Form) {Δ : Set Form} (mcs : Δ.MCS) (wit : Δ.witnessed) (mem : ◇φ ∈ Δ) :
-  (n : ℕ) → (∃ Γ : Set Form, Canonical.R Δ Γ ∧ φ ∈ Γ ∧ ∀ i : ℕ, i < n → Γ.has_wit_of (enum i))
+theorem set_family (enum : ℕ → Form N) {Δ : Set (Form N)} (mcs : Δ.MCS) (wit : Δ.witnessed) (mem : ◇φ ∈ Δ) :
+  (n : ℕ) → (∃ Γ : Set (Form N), Canonical.R Δ Γ ∧ φ ∈ Γ ∧ ∀ i : ℕ, i < n → Γ.has_wit_of (enum i))
   | 0     => by
       let Γ₀ := {φ} ∪ {ψ | □ψ ∈ Δ}
       have : Γ₀.consistent := by admit
@@ -100,7 +97,6 @@ theorem set_family (enum : ℕ → Form) {Δ : Set Form} (mcs : Δ.MCS) (wit : �
       have ⟨Γ_ih, ⟨R_ih, ⟨mem_ih, wit_ih⟩⟩⟩ := set_family enum mcs wit mem n
       admit
 
-def succesor_set (enum : ℕ → Form) {Δ : Set Form} (mcs : Δ.MCS) (wit : Δ.witnessed) (mem : ◇φ ∈ Δ) : Set Form :=
+def succesor_set (enum : ℕ → Form N) {Δ : Set (Form N)} (mcs : Δ.MCS) (wit : Δ.witnessed) (mem : ◇φ ∈ Δ) : Set (Form N) :=
   {φ | ∃ n : ℕ, φ ∈ (set_family enum mcs wit mem n).choose}
-
-theorem Completeness (Γ : Set Form) (φ : Form) : Γ ⊨ φ → Γ ⊢ φ := by admit  
+-/
