Hybrid/Form.lean
@@ -5,7 +5,11 @@ import Mathlib.Data.Fin.Basic
 import Mathlib.Logic.Equiv.Fin
 import Hybrid.Util
 
+open Classical
+
 section Basics
+  def TotalSet := {n : ℕ | True}
+
   structure PROP where
     letter : Nat
   deriving DecidableEq, Repr
@@ -14,22 +18,22 @@ section Basics
     letter : Nat
   deriving DecidableEq, Repr
 
-  structure NOM where
-    letter : Nat
+  structure NOM (N : Set ℕ) where
+    letter : N
   deriving DecidableEq, Repr
 
   instance : Max PROP where
     max := λ p => λ q => ite (p.letter > q.letter) p q
   instance svarmax : Max SVAR where
     max := λ x => λ y => ite (x.letter > y.letter) x y
-  instance : Max NOM where
+  instance : Max (NOM S) where
     max := λ i => λ j => ite (i.letter > j.letter) i j
 
-  theorem NOM_eq {i j : NOM} : (i = j) ↔ (i.letter = j.letter) := by
+  theorem NOM_eq {i j : NOM S} : (i = j) ↔ (i.letter = j.letter) := by
     cases i
     cases j
     simp
-  theorem NOM_eq' {i j : NOM} : (i = j) ↔ (j.letter = i.letter) := by
+  theorem NOM_eq' {i j : NOM S} : (i = j) ↔ (j.letter = i.letter) := by
     cases i
     cases j
     simp
@@ -37,8 +41,8 @@ section Basics
 
 --  instance ofNatSVAR : OfNat SVAR n    where
 --    ofNat := SVAR.mk n
-  instance : OfNat NOM n     where
-    ofNat := NOM.mk  n
+  instance : OfNat (NOM TotalSet) n     where
+    ofNat := NOM.mk  ⟨n, trivial⟩ 
   instance : Coe SVAR Nat  := ⟨SVAR.letter⟩
 --  instance : Coe NOM Nat   := ⟨NOM.letter⟩
   instance : Coe Nat SVAR  := ⟨SVAR.mk⟩   
@@ -47,69 +51,121 @@ section Basics
     le    := λ x => λ y =>  x.letter ≤ y.letter
   instance SVAR.lt : LT SVAR         where
     lt    := λ x => λ y =>  x.letter < y.letter
-  instance NOM.le : LE NOM         where
+  instance NOM.le : LE (NOM S)       where
     le    := λ x => λ y =>  x.letter ≤ y.letter
-  instance NOM.lt : LT NOM         where
+  instance NOM.lt : LT (NOM S)         where
     lt    := λ x => λ y =>  x.letter < y.letter
   instance SVAR.add : HAdd SVAR Nat SVAR where
-    hAdd  := λ x => λ n => SVAR.mk (x.letter + n)
-  instance NOM.add : HAdd NOM Nat NOM where
-    hAdd  := λ x => λ n => NOM.mk (x.letter + n)
-  instance : HMul NOM Nat NOM where
-    hMul  := λ x => λ n => NOM.mk (x.letter * n)
-  instance NOM.hmul : HMul Nat NOM NOM where
-    hMul  := λ n => λ x => NOM.mk (x.letter * n)
-  instance : HMul NOM ℕ ℕ where
+    hAdd  := λ x => λ n => (x.letter + n)
+  @[simp] instance NOM.add : HAdd (NOM TotalSet) Nat (NOM TotalSet) where
+    hAdd  := λ x => λ n => ⟨(x.letter + n), trivial⟩ 
+  @[simp] instance : HSub (NOM TotalSet) Nat (NOM TotalSet) where
+    hSub  := λ x => λ n => ⟨(x.letter - n), trivial⟩ 
+  @[simp] instance : HMul (NOM TotalSet) Nat (NOM TotalSet) where
+    hMul  := λ x => λ n => ⟨(x.letter * n), trivial⟩
+  @[simp] instance : HDiv (NOM TotalSet) Nat (NOM TotalSet) where
+    hDiv  := λ x => λ n => ⟨(x.letter / n), trivial⟩ 
+  @[simp] instance NOM.hmul : HMul Nat (NOM TotalSet) (NOM TotalSet) where
+    hMul  := λ n => λ x => ⟨(x.letter * n), trivial⟩
+  @[simp] instance : HMul (NOM TotalSet) ℕ ℕ where
     hMul  := λ x => λ n => x.letter * n
 
-  instance : IsTrans NOM GT.gt where
+  instance : IsTrans (NOM S) GT.gt where
     trans := λ _ _ _ h1 h2 => Nat.lt_trans h2 h1
 
-  instance : IsTotal NOM GE.ge where
-    total := by simp [NOM.le, Nat.le_total]
+  instance : IsTotal (NOM S) GE.ge where
+    total := by simp [NOM.le, LE.le, Nat.le_total]
 
-  instance : IsTrans NOM GE.ge where
+  instance : IsTrans (NOM S) GE.ge where
     trans := λ _ _ _ h1 h2 => Nat.le_trans h2 h1
 
-  theorem NOM.gt_iff_ge_and_ne {a b : NOM} : a > b ↔ (a ≥ b ∧ a ≠ b) := by
-    simp only [GT.gt, GE.ge, NOM.lt, NOM.le, NOM.mk, Nat.lt_iff_le_and_ne, ne_eq, NOM_eq']
+  theorem NOM.gt_iff_ge_and_ne {a b : (NOM S)} : a > b ↔ (a ≥ b ∧ a ≠ b) := by
+    simp only [GT.gt, GE.ge, NOM.lt, NOM.le, LE.le, LT.lt, NOM.mk, ne_eq, NOM_eq']
+    apply Iff.intro
+    . intro h
+      apply And.intro
+      . exact (Nat.lt_iff_le_and_ne.mp h).1
+      . have := (Nat.lt_iff_le_and_ne.mp h).2
+        intro habs
+        simp [habs] at this
+    . rw [←ne_eq]
+      intro ⟨h1, h2⟩
+      apply Nat.lt_iff_le_and_ne.mpr
+      apply And.intro
+      . exact h1
+      . intro habs
+        apply h2
+        apply Subtype.eq
+        assumption
 
-  inductive Form where
+  inductive Form (N : Set ℕ) where
     -- atomic formulas:
-    | bttm : Form
-    | prop : PROP → Form
-    | svar : SVAR → Form
-    | nom  :  NOM → Form
+    | bttm : Form N
+    | prop : PROP   → Form N
+    | svar : SVAR   → Form N
+    | nom  :  NOM N → Form N
     -- connectives:
-    | impl : Form → Form → Form
+    | impl : Form N → Form N → Form N
     -- modal:
-    | box  : Form → Form
+    | box  : Form N → Form N
     -- hybrid:
-    | bind : SVAR → Form → Form
+    | bind : SVAR → Form N → Form N
   deriving DecidableEq, Repr
 
-  def Form.depth : Form → ℕ
+  def Form.depth : Form N → ℕ
     | .impl φ ψ =>  1 + Form.depth φ + Form.depth ψ
     | .box  φ   =>  1 + Form.depth φ
     | .bind _ φ =>  2 + Form.depth φ
     | _       =>    0
 
   @[simp]
-  def Form.neg      : Form → Form := λ φ => Form.impl φ Form.bttm
+  def Form.neg      : Form N → Form N := λ φ => Form.impl φ Form.bttm
   @[simp]
-  def Form.conj     : Form → Form → Form := λ φ => λ ψ => Form.neg (Form.impl φ (Form.neg ψ))
+  def Form.conj     : Form N → Form N → Form N := λ φ => λ ψ => Form.neg (Form.impl φ (Form.neg ψ))
   @[simp]
-  def Form.iff      : Form → Form → Form := λ φ => λ ψ => Form.conj (Form.impl φ ψ) (Form.impl ψ φ) 
+  def Form.iff      : Form N → Form N → Form N := λ φ => λ ψ => Form.conj (Form.impl φ ψ) (Form.impl ψ φ) 
   @[simp]
-  def Form.disj     : Form → Form → Form := λ φ => λ ψ => Form.impl (Form.neg φ) ψ
+  def Form.disj     : Form N → Form N → Form N := λ φ => λ ψ => Form.impl (Form.neg φ) ψ
   @[simp]
-  def Form.diamond  : Form → Form := λ φ => Form.neg (Form.box (Form.neg φ))
+  def Form.diamond  : Form N → Form N := λ φ => Form.neg (Form.box (Form.neg φ))
   @[simp,match_pattern]
-  def Form.bind_dual: SVAR → Form → Form := λ x => λ φ => Form.neg (Form.bind x (Form.neg φ))
+  def Form.bind_dual: SVAR → Form N → Form N := λ x => λ φ => Form.neg (Form.bind x (Form.neg φ))
 
-  instance : Coe PROP Form  := ⟨Form.prop⟩
-  instance : Coe SVAR Form  := ⟨Form.svar⟩
-  instance : Coe NOM  Form  := ⟨Form.nom⟩
+  instance : Coe PROP     (Form N)  := ⟨Form.prop⟩
+  instance : Coe SVAR     (Form N)  := ⟨Form.svar⟩
+  instance : Coe (NOM N)  (Form N)  := ⟨Form.nom⟩
+
+  def Form.total : Form N → Form TotalSet
+    | .bttm     => Form.bttm
+    | .prop p   => Form.prop p
+    | .svar v   => Form.svar v
+    | .nom i    => Form.nom ⟨i.1.1, trivial⟩
+    | .impl ψ χ => Form.impl ψ.total χ.total
+    | .box ψ    => Form.box ψ.total
+    | .bind v ψ => Form.bind v ψ.total
+  
+  noncomputable def Form.total_inv : Form TotalSet → Option (Form N)
+    | .bttm     => some Form.bttm
+    | .prop p   => some p
+    | .svar v   => some v
+    | .nom i    => if h : i.1.1 ∈ N then
+                      Form.nom ⟨i.1.1, h⟩
+                    else none
+    | .impl ψ χ => 
+        match ψ.total_inv, χ.total_inv with
+        | some a, some b => some (Form.impl a b)
+        | _, _           => none
+    | .box ψ => 
+        match ψ.total_inv with
+        | some a => some (Form.box a)
+        | _      => none
+    | .bind v ψ => 
+        match ψ.total_inv with
+        | some a => some (Form.bind v a)
+        | _      => none
+
+  theorem is_inv {φ : Form N} : φ.total.total_inv = some φ := by
+    induction φ <;> simp [Form.total, Form.total_inv, *]
 
   infixr:60 "⟶" => Form.impl
   infixl:65 "⋀" => Form.conj
@@ -122,29 +178,107 @@ section Basics
   infixr:60 "⟷" => Form.iff
   notation "⊥"  => Form.bttm
 
-  def conjunction (Γ : Set Form) (L : List Γ) : Form :=
+  theorem total_inj {φ ψ : Form N} : φ.total = ψ.total → φ = ψ := by
+    induction φ generalizing ψ with
+    | impl a b ih1 ih2 =>
+          cases ψ with 
+          | impl c d => simp [Form.total, -implication_disjunction]
+                        intros
+                        apply And.intro <;> (first | apply ih1 | apply ih2) <;> assumption
+          | _    => simp [Form.total]
+    | box a ih | bind v a ih =>
+        cases ψ with
+        | box b    => simp [Form.total, -implication_disjunction]; try apply ih
+        | bind u b => simp [Form.total, -implication_disjunction];
+                      try (intro; simp only [*, true_and]; apply ih)
+        | _     => simp  [Form.total]
+    | _    => cases ψ <;> simp [Form.total, NOM_eq, -implication_disjunction] <;>
+                          (intros; apply Subtype.eq; assumption)
+
+  theorem total_impl {φ : Form N} {ψ_t χ_t : Form TotalSet} : φ.total = (ψ_t ⟶ χ_t) → ∃ ψ χ : Form N, φ = (ψ ⟶ χ) := by
+    intro eq
+    cases φ <;> simp [Form.total] at *
+  theorem total_impl' {φ : Form N} {ψ_t χ_t : Form TotalSet} : φ.total = (ψ_t ⟶ χ_t) →
+    match φ with
+    | .impl ψ χ => True
+    | _         => False := by
+      intro eq
+      split
+      . trivial
+      . next h =>
+          have ⟨ψ, χ, hw⟩ :=  total_impl eq
+          exact h ψ χ hw
+  theorem total_box {φ : Form N} {ψ_t : Form TotalSet} : φ.total = □ψ_t → ∃ ψ : Form N, φ = □ψ := by
+    intro eq
+    cases φ <;> simp [Form.total] at *
+  theorem total_box' {φ : Form N} {ψ_t : Form TotalSet} : φ.total = □ ψ_t →
+    match φ with
+    | .box ψ    => True
+    | _         => False := by
+      intro eq
+      split
+      . trivial
+      . next h =>
+          have ⟨ψ, hw⟩ :=  total_box eq
+          exact h ψ hw
+  theorem total_bind {φ : Form N} {ψ_t : Form TotalSet} : (φ.total = all v, ψ_t) → ∃ ψ : Form N, (φ = all v, ψ) := by
+    intro eq
+    cases φ <;> simp [Form.total] at *;
+                exact eq.left
+
+  theorem total_ax_k {φ : Form N} {ψ_t χ_t : Form TotalSet} : φ.total = □(ψ_t ⟶ χ_t) ⟶ (□ψ_t ⟶ □χ_t) →
+    ∃ ψ χ : Form N, φ = □(ψ ⟶ χ) ⟶ (□ψ ⟶ □χ) := by
+      intro eq
+      have ⟨l, r, hw⟩ := total_impl eq
+      simp [hw, Form.total] at eq 
+      have ⟨p, q⟩ := eq 
+      clear eq
+
+      have ⟨t, w1⟩  := total_box p
+      simp [w1, Form.total] at p
+      have ⟨a, b, n⟩   := total_impl p
+      rw [n] at w1
+      rw [w1] at hw
+      
+      have ⟨u, v, w2⟩  := total_impl q  
+      simp [w2, Form.total] at q
+      have ⟨c, m1⟩     := total_box q.1
+      have ⟨d, m2⟩     := total_box q.2
+      rw [m1, m2] at w2
+      rw [w2] at hw
+
+      simp [congrArg Form.total m1, congrArg Form.total m2, Form.total] at q
+      simp [congrArg Form.total n, Form.total] at p
+      rw [←p.1, ←p.2] at q
+      clear p
+
+      rw [total_inj q.1, total_inj q.2] at hw
+      exists a; exists b
+  
+  def conjunction (Γ : Set (Form N)) (L : List Γ) : Form N :=
   match L with
     | []     => ⊥ ⟶ ⊥
     | h :: t => h.val ⋀ conjunction Γ t
 
-  def Form.new_var  : Form → SVAR
+  def Form.new_var  : Form N → SVAR
   | .svar x   => x+1
   | .impl ψ χ => max (ψ.new_var) (χ.new_var)
   | .box  ψ   => ψ.new_var
   | .bind x ψ => max (x+1) (ψ.new_var)
   | _         => ⟨0⟩
 
-  def Form.new_nom  : Form → NOM
+
+  def Form.new_nom  : Form TotalSet → NOM TotalSet
   | .nom  i   => i+1
   | .impl ψ χ => max (ψ.new_nom) (χ.new_nom)
   | .box  ψ   => ψ.new_nom
   | .bind _ ψ => ψ.new_nom
-  | _         => ⟨0⟩ 
+  | _         => ⟨0, trivial⟩ 
 
 end Basics
 
 section Substitutions
-  def occurs (x : SVAR) (φ : Form) : Bool :=
+  def occurs (x : SVAR) (φ : Form N) : Bool :=
     match φ with
     | Form.bttm     => false
     | Form.prop _   => false
@@ -154,7 +288,7 @@ section Substitutions
     | Form.box  φ   => occurs x φ
     | Form.bind _ φ => occurs x φ
 
-  def is_free (x : SVAR) (φ : Form) : Bool :=
+  def is_free (x : SVAR) (φ : Form N) : Bool :=
     match φ with
     | Form.bttm     => false
     | Form.prop _   => false
@@ -164,12 +298,12 @@ section Substitutions
     | Form.box  φ   => is_free x φ
     | Form.bind y φ => (y != x) && (is_free x φ)
 
-  def is_bound (x : SVAR) (φ : Form) := (occurs x φ) && !(is_free x φ)
+  def is_bound (x : SVAR) (φ : Form N) := (occurs x φ) && !(is_free x φ)
   
   -- conventions for substitutions can get confusing
   -- "φ[s // x], the formula obtained by substituting s for all *free* occurrences of x in φ"
   -- for reference: Blackburn 1998, pg. 628
-  def subst_svar (φ : Form) (s : SVAR) (x : SVAR) : Form :=
+  def subst_svar (φ : Form N) (s : SVAR) (x : SVAR) : Form N :=
     match φ with
     | Form.bttm     => φ
     | Form.prop _   => φ
@@ -179,7 +313,7 @@ section Substitutions
     | Form.box  φ   => □ (subst_svar φ s x)
     | Form.bind y φ => ite (x = y) (Form.bind y φ) (Form.bind y (subst_svar φ s x))
 
-  def subst_nom (φ : Form) (s : NOM) (x : SVAR) : Form :=
+  def subst_nom (φ : Form N) (s : NOM N) (x : SVAR) : Form N :=
     match φ with
     | Form.bttm     => φ
     | Form.prop _   => φ
@@ -189,7 +323,7 @@ section Substitutions
     | Form.box  φ   => □ (subst_nom φ s x)
     | Form.bind y φ => ite (x = y) (Form.bind y φ) (Form.bind y (subst_nom φ s x))
 
-  def is_substable (φ : Form) (y : SVAR) (x : SVAR) : Bool :=
+  def is_substable (φ : Form N) (y : SVAR) (x : SVAR) : Bool :=
     match φ with
     | Form.bttm     => true
     | Form.prop _   => true
@@ -216,21 +350,14 @@ end Substitutions
 
 section NominalSubstitution 
 
-  def Form.nominals : Form → List NOM
-  | .nom a      => [a]
-  | .impl φ ψ   => φ.nominals ++ ψ.nominals
-  | .box φ      => φ.nominals
-  | .bind _ φ   => φ.nominals
-  | _           => []
-
-  def nom_subst_nom : Form → NOM → NOM → Form
+  def nom_subst_nom : Form N → NOM N → NOM N → Form N
   | .nom a, i, j     => if a = j then i else a
   | .impl φ ψ, i, j  => nom_subst_nom φ i j ⟶ nom_subst_nom ψ i j
   | .box φ, i, j     => □ nom_subst_nom φ i j
   | .bind y φ, i, j  => all y, nom_subst_nom φ i j
   | φ, _, _          => φ
 
-  def nom_subst_svar : Form → SVAR → NOM → Form
+  def nom_subst_svar : Form N → SVAR → NOM N → Form N
   | .nom a, i, j     => if a = j then i else a
   | .impl φ ψ, i, j  => nom_subst_svar φ i j ⟶ nom_subst_svar ψ i j
   | .box φ, i, j     => □ nom_subst_svar φ i j
@@ -240,14 +367,14 @@ section NominalSubstitution
   notation:150 φ "[" i "//" a "]" => nom_subst_nom φ i a
   notation:150 φ "[" i "//" a "]" => nom_subst_svar φ i a
 
-  def nom_occurs : NOM → Form → Bool
+  def nom_occurs : NOM N → Form N → Bool
   | i, .nom j    => i = j
   | i, .impl ψ χ => (nom_occurs i ψ) || (nom_occurs i χ)
   | i, .box ψ    => nom_occurs i ψ
   | i, .bind _ ψ => nom_occurs i ψ
   | _, _         => false
 
-  def all_nocc (i : NOM) (Γ : Set Form) := ∀ (φ : Form), φ ∈ Γ → nom_occurs i φ = false
+  def all_nocc (i : NOM N) (Γ : Set (Form N)) := ∀ (φ : Form N), φ ∈ Γ → nom_occurs i φ = false
 
   theorem all_noc_conj (h : all_nocc i Γ) (L : List Γ) : nom_occurs i (conjunction Γ L) = false := by
     induction L with
@@ -256,27 +383,27 @@ section NominalSubstitution
         simp [conjunction, nom_occurs, ih, -Form.conj]
         exact h head head.2
 
-  def Form.bulk_subst : Form → List NOM → List NOM → Form
+  def Form.bulk_subst : Form N → List (NOM N) → List (NOM N) → Form N
   | φ, h₁ :: t₁, h₂ :: t₂ => bulk_subst (φ[h₁ // h₂]) t₁ t₂
   | φ, _, []    =>  φ
   | φ, [], _    =>  φ
 
-  def Form.list_noms : Form → List NOM
+  def Form.list_noms : (Form N) → List (NOM N)
   | nom  i   => [i]
   | impl φ ψ => (List.merge GE.ge φ.list_noms ψ.list_noms).dedup
   | box φ    => φ.list_noms
   | bind _ φ => φ.list_noms
   | _        => []
 
-  def Form.odd_list_noms : Form → List NOM := λ φ => φ.list_noms.map (λ i => 2*i+1)
+  def Form.odd_list_noms : Form TotalSet → List (NOM TotalSet) := λ φ => φ.list_noms.map (λ i => 2*i+1)
 
-  def Form.odd_noms : Form → Form := λ φ => φ.bulk_subst φ.odd_list_noms φ.list_noms
+  def Form.odd_noms : Form TotalSet → Form TotalSet := λ φ => φ.bulk_subst φ.odd_list_noms φ.list_noms
 
-  def Set.odd_noms : Set Form → Set Form := λ Γ => {Form.odd_noms φ | φ ∈ Γ} 
+  def Set.odd_noms : Set (Form TotalSet) → Set (Form TotalSet) := λ Γ => {Form.odd_noms φ | φ ∈ Γ} 
 
-  def nocc_bulk_property (l1 l2 : List NOM) (φ : Form) := ∀ {n : Fin l1.length} {i : NOM}, (i = l1[n]) → (i ∉ φ.list_noms ∨ i ∈ l2.take n) ∧ i ∉ l1.take n
+  def nocc_bulk_property (l1 l2 : List (NOM TotalSet)) (φ : Form TotalSet) := ∀ {n : Fin l1.length} {i : NOM TotalSet}, (i = l1[n]) → (i ∉ φ.list_noms ∨ i ∈ l2.take n) ∧ i ∉ l1.take n
 
-  theorem list_noms_sorted_ge {φ : Form} : φ.list_noms.Sorted GE.ge := by
+  theorem list_noms_sorted_ge {φ : Form N} : φ.list_noms.Sorted GE.ge := by
     induction φ with
     | nom  i   => simp [Form.list_noms]
     | impl φ ψ ih1 ih2 =>
@@ -285,16 +412,16 @@ section NominalSubstitution
     | bind _ _ ih => exact ih
     | _        => simp [Form.list_noms]
   
-  theorem list_noms_nodup {φ : Form} : φ.list_noms.Nodup := by
+  theorem list_noms_nodup {φ : Form N} : φ.list_noms.Nodup := by
     induction φ <;> simp [Form.list_noms, List.nodup_dedup, *]
 
-  theorem list_noms_sorted_gt {φ : Form} : φ.list_noms.Sorted GT.gt := by
+  theorem list_noms_sorted_gt {φ : Form N} : φ.list_noms.Sorted GT.gt := by
     simp [List.Sorted, List.Pairwise, GT.gt, NOM.gt_iff_ge_and_ne]
     apply List.Pairwise.and
     apply list_noms_nodup
     apply list_noms_sorted_ge
 
-  theorem list_noms_chain' {φ : Form} : φ.list_noms.Chain' GT.gt := by
+  theorem list_noms_chain' {φ : Form N} : φ.list_noms.Chain' GT.gt := by
     rw [List.chain'_iff_pairwise]
     exact list_noms_sorted_gt
 
@@ -305,8 +432,8 @@ section IteratedModalities
   -- Axiom utils. Since we won't be assuming a transitive frame,
   -- it will make sense to be able to construct formulas with
   -- iterated modal operators at their beginning (ex., for axiom nom)
-  def iterate_nec (n : Nat) (φ : Form) : Form :=
-    let rec loop : Nat → Form → Form
+  def iterate_nec (n : Nat) (φ : Form N) : Form N :=
+    let rec loop : Nat → Form  N → Form N
       | 0, φ   => φ
       | n+1, φ => □ (loop n φ)
     loop n φ
@@ -330,8 +457,8 @@ section IteratedModalities
 
 
 
-  def iterate_pos (n : Nat) (φ : Form) : Form :=
-    let rec loop : Nat → Form → Form
+  def iterate_pos (n : Nat) (φ : Form N) : Form N :=
+    let rec loop : Nat → Form N → Form N
       | 0, φ   => φ
       | n+1, φ => ◇ (loop n φ)
     loop n φ
