Hybrid/Proof.lean
@@ -1,64 +1,71 @@
 import Hybrid.Form
 import Hybrid.Tautology
 
-inductive Proof : Form → Prop where
+inductive Proof : Form N → Type where
   -- Deduction rules:
 
   -- if φ is a theorem, ∀ v, φ is a theorem
-  | general {φ : Form} (v : SVAR):
+  | general {φ : Form N} (v : SVAR):
         Proof φ → Proof (all v, φ)
 
   -- if φ is a theorem, □ φ is a theorem 
-  | necess {φ : Form}:
+  | necess {φ : Form N}:
         Proof φ → Proof (□ φ)
 
   -- modus ponens:
-  | mp {φ ψ : Form}:
+  | mp {φ ψ : Form N}:
         Proof (φ ⟶ ψ) → Proof φ → Proof ψ
 
   -- All propositional tautologies
-  | tautology {φ : Form}:
+  | tautology {φ : Form N}:
         Tautology φ → Proof φ
 
   -- Axioms for modal + hybrid logic:
   -- distribution schema (axiom K)
-  | ax_k {φ ψ : Form}:
+  | ax_k {φ ψ : Form N}:
         Proof (□ (φ ⟶ ψ) ⟶ (□ φ ⟶ □ ψ))
 
-  | ax_q1 (φ ψ : Form) {v : SVAR} (p : is_free v φ = false):
+  | ax_q1 (φ ψ : Form N) {v : SVAR} (p : is_free v φ = false):
         Proof ((all v, φ ⟶ ψ) ⟶ (φ ⟶ all v, ψ))
 
   -- two different instances of Axiom Q2: one for SVAR, one for NOM
-  | ax_q2_svar (φ : Form) (v s : SVAR) (p : is_substable φ s v):
+  | ax_q2_svar (φ : Form N) (v s : SVAR) (p : is_substable φ s v):
       Proof ((all v, φ) ⟶ φ[s // v])
 
-  | ax_q2_nom (φ : Form) (v : SVAR) (s : NOM):
+  | ax_q2_nom (φ : Form N) (v : SVAR) (s : NOM N):
       Proof ((all v, φ) ⟶ φ[s // v])
 
   | ax_name (v : SVAR):
       Proof (ex v, v)
 
-  | ax_nom {φ : Form} {v : SVAR} (m n : Nat):
+  | ax_nom {φ : Form N} {v : SVAR} (m n : Nat):
       Proof (all v, (iterate_pos m (v ⋀ φ) ⟶ iterate_nec n (v ⟶ φ)))
 
-  | ax_brcn {φ : Form} {v : SVAR}:
+  | ax_brcn {φ : Form N} {v : SVAR}:
       Proof ((all v, □ φ) ⟶ (□ all v, φ))
 
-def SyntacticConsequence (Γ : Set Form) (φ : Form) : Prop := ∃ L, Proof ((conjunction Γ L) ⟶ φ)  
+def Proof.size : Proof φ → ℕ
+  | .general _ pf => pf.size + 1
+  | .necess pf    => pf.size + 1
+  | .mp pf1 pf2   => pf1.size + pf2.size + 1
+  | _ => 1
+
+def SyntacticConsequence (Γ : Set (Form N)) (φ : Form N) := Σ L, Proof ((conjunction Γ L) ⟶ φ)
 
 prefix:500 "⊢"  => Proof
 infix:500 "⊢"   => SyntacticConsequence
 
-notation "⊬" φ    => ¬(Proof φ)
-notation Γ "⊬" φ  => ¬(SyntacticConsequence Γ φ)
+notation "⊬" φ    => (Proof φ) → False
+notation Γ "⊬" φ  => (SyntacticConsequence Γ φ) → False
 
-def Set.consistent (Γ : Set Form) := Γ ⊬ ⊥
 
-def Set.MCS (Γ : Set Form) := Γ.consistent ∧ (∀ {φ : Form}, (¬φ ∈ Γ) → ((Γ ∪ {φ}) ⊢ ⊥))
+def consistent (Γ : Set (Form N)) := ∀ (_ : SyntacticConsequence Γ ⊥), False
 
-def Set.witnessed (Γ : Set Form) : Prop := ∀ {φ : Form},
+def MCS (Γ : Set (Form N)) := consistent Γ ∧ (∀ {φ : Form N}, (¬φ ∈ Γ) → ¬consistent (Γ ∪ {φ}))
+
+def witnessed (Γ : Set (Form N)) : Prop := ∀ {φ : Form N},
   φ ∈ Γ → 
     match φ with 
 --      | ex x, ψ => ∃ i : NOM, ((ex x, ψ) ⟶ ψ[i // x]) ∈ Γ
-      | ex x, ψ => ∃ i : NOM, ψ[i // x] ∈ Γ 
+      | ex x, ψ => ∃ i : NOM N, ψ[i // x] ∈ Γ 
       | _   => φ ∈ Γ
