Hybrid/ProofUtils.lean
@@ -4,20 +4,16 @@ import Hybrid.ListUtils
 
 namespace Proof
 
-theorem iff_mp (h : ⊢ (φ ⟷ ψ)) : ⊢ (φ ⟶ ψ) := by
-  rw [Form.iff] at h
-  have := tautology (@conj_elim_l (φ ⟶ ψ) (ψ ⟶ φ))
-  exact mp this h
+theorem iff_mp (h : ⊢ (φ ⟷ ψ)) : ⊢ (φ ⟶ ψ) :=
+  mp (tautology conj_elim_l) h
 
-theorem iff_mpr (h : ⊢ (φ ⟷ ψ)) : ⊢ (ψ ⟶ φ) := by
-  rw [Form.iff] at h
-  have := tautology (@conj_elim_r (φ ⟶ ψ) (ψ ⟶ φ))
-  exact mp this h
+theorem iff_mpr (h : ⊢ (φ ⟷ ψ)) : ⊢ (ψ ⟶ φ) :=
+  mp (tautology conj_elim_r) h
 
-theorem hs (h1 : ⊢ (φ ⟶ ψ)) (h2 : ⊢ (ψ ⟶ χ)) : ⊢ (φ ⟶ χ) := by
-  exact mp (mp (tautology hs_taut) h1) h2
+theorem hs (h1 : ⊢ (φ ⟶ ψ)) (h2 : ⊢ (ψ ⟶ χ)) : ⊢ (φ ⟶ χ) :=
+  mp (mp (tautology hs_taut) h1) h2
 
-theorem rename_bound (h1 : occurs y φ = false) (h2 : is_substable φ y x) : ⊢ ((all x, φ) ⟷ all y, φ[y // x]) := by
+theorem rename_bound {φ : Form N} (h1 : occurs y φ = false) (h2 : is_substable φ y x) : ⊢ ((all x, φ) ⟷ all y, φ[y // x]) := by
   rw [Form.iff]
   apply mp
   . apply mp
@@ -34,11 +30,11 @@ theorem rename_bound (h1 : occurs y φ = false) (h2 : is_substable φ y x) : ⊢
     have l3 := general x l1
     by_cases xy : x = y
     . rw [←xy] at h1
-      have notf := preserve_notfree x y (notoccurs_notfree (@notocc_beforeafter_subst φ x y h1))
+      have notf := preserve_notfree x y (notoccurs_notfree (@notocc_beforeafter_subst N φ x y h1))
       have l4 := ax_q1 (all y, φ[y//x]) φ notf
       have l5 := mp l4 l3
       exact l5
-    . have notf := preserve_notfree x y (@notfree_after_subst φ x y xy)
+    . have notf := preserve_notfree x y (@notfree_after_subst N φ x y xy)
       have l4 := ax_q1 (all y, φ[y//x]) φ notf
       have l5 := mp l4 l3
       exact l5
@@ -58,15 +54,13 @@ theorem rename_bound_ex (h1 : occurs y φ = false) (h2 : is_substable φ y x) : 
 -- Quite bothersome to work with subtypes and coerce properly.
 -- The code looks ugly, but in essence it follows the proof given
 -- in LaTeX.
-theorem Deduction (Γ : Set Form) : Γ ⊢ (ψ ⟶ φ) ↔ (Γ ∪ {ψ}) ⊢ φ := by
-  apply Iff.intro
+theorem Deduction {Γ : Set (Form N)} : Γ ⊢ (ψ ⟶ φ) iff (Γ ∪ {ψ}) ⊢ φ := by
+  apply TypeIff.intro
   . intro h
     match h with
     | ⟨L, hpf⟩ =>
-        have t_com12 := tautology (@com12 (conjunction Γ L) ψ φ)
-        have l1 := mp t_com12 hpf
-        have t_imp := tautology (@imp ψ (conjunction Γ L) φ)
-        have l2 := mp t_imp l1
+        have l1 := mp (tautology com12) hpf
+        have l2 := mp (tautology imp) l1
         have pfmem : ψ ∈ Γ ∪ {ψ} := by simp
         let L' : List ↑(Γ ∪ {ψ}) := ⟨ψ, pfmem⟩ :: list_convert L
         rw [conj_incl] at l2
@@ -74,16 +68,14 @@ theorem Deduction (Γ : Set Form) : Γ ⊢ (ψ ⟶ φ) ↔ (Γ ∪ {ψ}) ⊢ φ 
   . intro h
     match h with
     | ⟨L', hpf⟩ =>
-      have t_ax1 := tautology (@ax_1 (conjunction (Γ ∪ {ψ}) L'⟶φ) ψ)
+      have t_ax1 := tautology (@ax_1 N (conjunction (Γ ∪ {ψ}) L'⟶φ) ψ)
       have l1 := mp t_ax1 hpf
-      have t_com12 := tautology (@com12 ψ (conjunction (Γ ∪ {ψ}) L') φ)
-      have l2 := mp t_com12 l1
+      have l2 := mp (tautology com12) l1
       by_cases elem : elem' L' ψ
       . have t_help := tautology (deduction_helper L' ψ (ψ⟶φ) elem)
         have l3 := mp t_help l2
-        have t_idem := tautology (@idem (conjunction (Γ ∪ {ψ}) (filter' L' ψ)) ψ φ)
-        have l4 := mp t_idem l3
-        have not_elem_L' := eq_false_of_ne_true (@filter'_filters Γ ψ L')
+        have l4 := mp (tautology idem) l3
+        have not_elem_L' := eq_false_of_ne_true (@filter'_filters N Γ ψ L')
         let L : List Γ := list_convert_rev (filter' L' ψ) not_elem_L'
         rw [conj_incl_rev (filter' L' ψ) not_elem_L'] at l4
         exact ⟨L, l4⟩ 
@@ -101,9 +93,9 @@ lemma increasing_consequence (h1 : Γ ⊢ φ) (h2 : Γ ⊆ Δ) : Δ ⊢ φ := by
   rw [conj_incl_general h2 L] at pf
   exact pf
 
-theorem Γ_empty : ∅ ⊢ φ ↔ ⊢ φ := by
+theorem Γ_empty {φ : Form N} : ∅ ⊢ φ iff ⊢ φ := by
   unfold SyntacticConsequence
-  apply Iff.intro
+  apply TypeIff.intro
   . intro pf
     have ⟨L, pf⟩ := pf
     have := empty_list L
@@ -116,7 +108,7 @@ theorem Γ_empty : ∅ ⊢ φ ↔ ⊢ φ := by
       exact this
     . exact pf
   . intro pf
-    let L : List ↑{x : Form | False} := []
+    let L : List ↑{x : Form N | False} := []
     exists L
     simp [conjunction]
     apply mp
@@ -132,38 +124,39 @@ theorem Γ_theorem : ⊢ φ → (∀ Γ, Γ ⊢ φ) := by
 
 theorem Γ_theorem_rev : (∀ Γ, Γ ⊢ φ) → ⊢ φ := by
   intro h
-  rw [←Γ_empty]
+  apply Γ_empty.mp
   apply h
 
-theorem Γ_theorem_iff : ⊢ φ ↔ (∀ Γ, Γ ⊢ φ) := by
-  apply Iff.intro <;> first | apply Γ_theorem | apply Γ_theorem_rev
+theorem Γ_theorem_iff : ⊢ φ iff (∀ Γ, Γ ⊢ φ) := by
+  apply TypeIff.intro <;> first | apply Γ_theorem | apply Γ_theorem_rev
 
 theorem Γ_premise : φ ∈ Γ → Γ ⊢ φ := by
   intro mem
   have : Γ = Γ ∪ {φ} := by simp [mem]
-  rw [this, ←Deduction]
+  rw [this]
+  apply Deduction.mp
   apply Γ_theorem
   apply tautology
   eval
 
-theorem Γ_mp_helper1 {Γ : Set Form} (φ ψ χ : Form) : (Γ ⊢ ((φ ⋀ ψ) ⟶ χ)) ↔ ((Γ ∪ {φ}) ⊢ (ψ ⟶ χ)) := by
-  apply Iff.intro
+theorem Γ_mp_helper1 {Γ : Set (Form N)} {φ ψ χ : Form N} : (Γ ⊢ ((φ ⋀ ψ) ⟶ χ)) iff ((Γ ∪ {φ}) ⊢ (ψ ⟶ χ)) := by
+  apply TypeIff.intro
   . intro h
     match h with
     | ⟨L, hL⟩ =>
         have l1 := hs hL (tautology exp)
         have l2 : Γ ⊢ (φ ⟶ ψ ⟶ χ) := ⟨L, l1⟩
-        rw [Deduction] at l2
-        exact l2
+        have l3 := Deduction.mp l2
+        exact l3
   . intro h
-    rw [←Deduction] at h
+    have h := Deduction.mpr h
     match h with
     | ⟨L, hL⟩ =>
         have l1 := hs hL (tautology imp)
         have l2 : Γ ⊢ (φ ⋀ ψ ⟶ χ) := ⟨L, l1⟩
         exact l2
 
-theorem Γ_mp_helper2 {Γ : Set Form} {L : List Γ} (h : Γ⊢(conjunction Γ L⟶ψ)) : Γ ⊢ ψ := by
+theorem Γ_mp_helper2 {Γ : Set (Form N)} {L : List Γ} (h : Γ⊢(conjunction Γ L⟶ψ)) : Γ ⊢ ψ := by
   induction L with
   | nil =>
       rw [conjunction] at h
@@ -172,7 +165,7 @@ theorem Γ_mp_helper2 {Γ : Set Form} {L : List Γ} (h : Γ⊢(conjunction Γ L�
       have l2 := mp (tautology (imp_taut imp_refl)) l1
       exists L
   | cons head tail ih =>
-      rw [conjunction, Γ_mp_helper1] at h
+      have h := Γ_mp_helper1.mp h
       have : (Γ ∪ {↑head}) = Γ := by simp [head.2]
       rw [this] at h
       exact ih h
@@ -186,57 +179,57 @@ theorem Γ_mp (h1: Γ ⊢ (φ ⟶ ψ)) (h2 : Γ ⊢ φ) : Γ ⊢ ψ := by
         have : Γ ⊢ (conjunction Γ L2⟶ψ) := ⟨L1, this⟩
         exact Γ_mp_helper2 this
 
-theorem Γ_neg_intro (h1 : Γ ⊢ (φ ⟶ ψ)) (h2 : Γ ⊢ (φ ⟶ ∼ψ)) : Γ ⊢ (∼φ) := by
-  have l1 := tautology (@neg_intro φ ψ)
+theorem Γ_neg_intro {φ : Form N} (h1 : Γ ⊢ (φ ⟶ ψ)) (h2 : Γ ⊢ (φ ⟶ ∼ψ)) : Γ ⊢ (∼φ) := by
+  have l1 := tautology (@neg_intro N φ ψ)
   have l2 := Γ_theorem l1 Γ
   have l3 := Γ_mp l2 h1
   have l4 := Γ_mp l3 h2
   exact l4
 
-theorem Γ_neg_elim (h : Γ ⊢ (∼∼φ)) : Γ ⊢ φ := by
-  have l1 := tautology (@dne φ)
+theorem Γ_neg_elim {φ : Form N} {φ : Form N} (h : Γ ⊢ (∼∼φ)) : Γ ⊢ φ := by
+  have l1 := tautology (@dne N φ)
   have l2 := Γ_theorem l1 Γ
   have l3 := Γ_mp l2 h
   exact l3
 
-theorem Γ_conj_intro (h1 : Γ ⊢ φ) (h2 : Γ ⊢ ψ) : Γ ⊢ (φ ⋀ ψ) := by
-  have l1 := tautology (@conj_intro φ ψ)
+theorem Γ_conj_intro {φ : Form N} (h1 : Γ ⊢ φ) (h2 : Γ ⊢ ψ) : Γ ⊢ (φ ⋀ ψ) := by
+  have l1 := tautology (@conj_intro N φ ψ)
   have l2 := Γ_theorem l1 Γ
   have l3 := Γ_mp l2 h1
   have l4 := Γ_mp l3 h2
   exact l4
 
-theorem Γ_conj_elim_l (h : Γ ⊢ (φ ⋀ ψ)) : Γ ⊢ φ := by
-  have l1 := tautology (@conj_elim_l φ ψ)
+theorem Γ_conj_elim_l {φ : Form N} (h : Γ ⊢ (φ ⋀ ψ)) : Γ ⊢ φ := by
+  have l1 := tautology (@conj_elim_l N φ ψ)
   have l2 := Γ_theorem l1 Γ
   have l3 := Γ_mp l2 h 
   exact l3
 
-theorem Γ_conj_elim_r (h : Γ ⊢ (φ ⋀ ψ)) : Γ ⊢ ψ := by
-  have l1 := tautology (@conj_elim_r φ ψ)
+theorem Γ_conj_elim_r {φ : Form N} (h : Γ ⊢ (φ ⋀ ψ)) : Γ ⊢ ψ := by
+  have l1 := tautology (@conj_elim_r N φ ψ)
   have l2 := Γ_theorem l1 Γ
   have l3 := Γ_mp l2 h 
   exact l3
 
-theorem Γ_disj_intro_l (h : Γ ⊢ φ) : Γ ⊢ (φ ⋁ ψ) := by
-  have l1 := tautology (@disj_intro_l φ ψ)
+theorem Γ_disj_intro_l {φ : Form N} (h : Γ ⊢ φ) : Γ ⊢ (φ ⋁ ψ) := by
+  have l1 := tautology (@disj_intro_l N φ ψ)
   have l2 := Γ_theorem l1 Γ
   exact Γ_mp l2 h
 
-theorem Γ_disj_intro_r (h : Γ ⊢ φ) : Γ ⊢ (ψ ⋁ φ) := by
-  have l1 := tautology (@disj_intro_r φ ψ)
+theorem Γ_disj_intro_r {φ : Form N} (h : Γ ⊢ φ) : Γ ⊢ (ψ ⋁ φ) := by
+  have l1 := tautology (@disj_intro_r N φ ψ)
   have l2 := Γ_theorem l1 Γ
   exact Γ_mp l2 h
 
-theorem Γ_disj_elim (h1 : Γ ⊢ (φ ⋁ ψ)) (h2 : Γ ⊢ (φ ⟶ χ)) (h3 : Γ ⊢ (ψ ⟶ χ)) : Γ ⊢ χ := by
-  have l1 := tautology (@disj_elim φ ψ χ)
+theorem Γ_disj_elim {φ : Form N} (h1 : Γ ⊢ (φ ⋁ ψ)) (h2 : Γ ⊢ (φ ⟶ χ)) (h3 : Γ ⊢ (ψ ⟶ χ)) : Γ ⊢ χ := by
+  have l1 := tautology (@disj_elim N φ ψ χ)
   have l2 := Γ_theorem l1 Γ
   have l3 := Γ_mp l2 h1
   have l4 := Γ_mp l3 h2
   have l5 := Γ_mp l4 h3
   exact l5
 
-theorem Γ_univ_intro {Γ : Set Form} {φ : Form} (h1 : ∀ ψ : Γ, is_free x ψ = false) (h2 : occurs y φ = false) (h3 : is_substable φ y x) : Γ ⊢ φ → Γ ⊢ (all y, φ[y // x]) := by
+theorem Γ_univ_intro {Γ : Set (Form N)} {φ : Form N} (h1 : ∀ ψ : Γ, is_free x ψ.1 = false) (h2 : occurs y φ = false) (h3 : is_substable φ y x) : Γ ⊢ φ → Γ ⊢ (all y, φ[y // x]) := by
   intro Γ_pf_φ
   match Γ_pf_φ with
   | ⟨L, l1⟩ =>
@@ -248,7 +241,7 @@ theorem Γ_univ_intro {Γ : Set Form} {φ : Form} (h1 : ∀ ψ : Γ, is_free x �
       have l6 := hs l4 l5
       exact ⟨L, l6⟩
 
-theorem Γ_univ_intro' {Γ : Set Form} {φ : Form} (h1 : ∀ ψ : Γ, is_free x ψ = false) : Γ ⊢ φ → Γ ⊢ (all x, φ) := by
+theorem Γ_univ_intro' {Γ : Set (Form N)} {φ : Form N} (h1 : ∀ ψ : Γ, is_free x ψ.1 = false) : Γ ⊢ φ → Γ ⊢ (all x, φ) := by
   intro Γ_pf_φ
   match Γ_pf_φ with
   | ⟨L, l1⟩ =>
@@ -258,11 +251,11 @@ theorem Γ_univ_intro' {Γ : Set Form} {φ : Form} (h1 : ∀ ψ : Γ, is_free x 
       have l4 := mp l3 l2
       exists L
 
-theorem dn_equiv_premise : Γ ⊢ (∼∼φ) ↔ Γ ⊢ φ := by
-  have l1 := tautology (@dne φ)
-  have l2 := tautology (@dni φ)
+theorem dn_equiv_premise {φ : Form N} : Γ ⊢ (∼∼φ) iff Γ ⊢ φ := by
+  have l1 := tautology (@dne N φ)
+  have l2 := tautology (@dni N φ)
   rw [SyntacticConsequence, SyntacticConsequence]
-  apply Iff.intro
+  apply TypeIff.intro
   repeat (
     intro ⟨L, _⟩;
     exists L;
@@ -272,7 +265,7 @@ theorem dn_equiv_premise : Γ ⊢ (∼∼φ) ↔ Γ ⊢ φ := by
 
 section Nominals
 
-theorem generalize_constants {φ : Form} {x : SVAR} (i : NOM) (h : x ≥ φ.new_var) : ⊢ φ → ⊢ (all x, φ[x // i]) := by
+theorem generalize_constants {φ : Form N} {x : SVAR} (i : NOM N) (h : x ≥ φ.new_var) : ⊢ φ → ⊢ (all x, φ[x // i]) := by
     intro pf
     apply general x
     induction pf generalizing x with
@@ -280,8 +273,8 @@ theorem generalize_constants {φ : Form} {x : SVAR} (i : NOM) (h : x ≥ φ.new_
         apply tautology
         simp [Tautology] at ht ⊢
         intro e
-        let f'  : Form → Bool := λ φ => if (e.f <| φ[x//i]) then true else false
-        let e'  : Eval := ⟨f', by simp [e.p1, nom_subst_svar], by simp [e.p2, nom_subst_svar]⟩
+        let f'  : Form N → Bool := λ φ => if (e.f <| φ[x//i]) then true else false
+        let e'  : Eval N := ⟨f', by simp [e.p1, nom_subst_svar], by simp [e.p2, nom_subst_svar]⟩
         rw [show ((e.f <| φ[x//i]) ↔ e'.f φ) by simp]
         exact ht e'
     | @general φ v _ ih   =>
@@ -295,7 +288,7 @@ theorem generalize_constants {φ : Form} {x : SVAR} (i : NOM) (h : x ≥ φ.new_
           exact general v (ih h)
     | @necess   ψ _ ih     =>  
         simp only [nom_subst_svar, occurs] at h ⊢
-        exact @necess (ψ[x//i]) (ih h)
+        apply necess; apply ih; assumption
     | @mp φ ψ _ _ ih1 ih2  =>
         simp only [occurs, Bool.or_eq_false_eq_eq_false_and_eq_false, not_and,
           Bool.not_eq_false] at ih1
@@ -313,16 +306,16 @@ theorem generalize_constants {φ : Form} {x : SVAR} (i : NOM) (h : x ≥ φ.new_
         have ih2 := ih2 ih2_cond
         rw [nom_subst_svar] at ih1
         have l1  := general y (mp ih1 ih2)
-        have l2  := @ax_q2_svar (ψ[y//i]) y x (new_var_subst h)
+        have l2  := ax_q2_svar (ψ[y//i]) y x (new_var_subst h)
         have l3  := mp l2 l1
         rw [nom_subst_trans i x y sub_cond] at l3
         exact l3
     | @ax_k φ ψ            =>
         simp only [nom_subst_svar]
-        exact @ax_k (φ[x//i]) (ψ[x//i])
+        apply ax_k
     | @ax_q1 φ ψ v h2       =>
         simp only [nom_subst_svar]
-        apply @ax_q1 (φ[x//i]) (ψ[x//i]) v
+        apply ax_q1
         have := new_var_geq2 (new_var_geq1 h).left
         have ha : x ≥ φ.new_var := (new_var_geq1 this.right).left
         have hb : v ≠ x := diffsvar this.left
@@ -344,7 +337,7 @@ theorem generalize_constants {φ : Form} {x : SVAR} (i : NOM) (h : x ≥ φ.new_
         by_cases ji : j = i
         . rw [ji] at h ⊢ 
           have f2 := (new_var_geq2 (new_var_geq1 h).left).right
-          have f1 := @new_var_subst'' φ x v f2
+          have f1 := @new_var_subst'' N φ x v f2
           have := new_var_subst' i f1 f2 f3
           have := ax_q2_svar (φ[x//i]) v x this
           rw [subst_collect_all]
@@ -352,55 +345,86 @@ theorem generalize_constants {φ : Form} {x : SVAR} (i : NOM) (h : x ≥ φ.new_
         . rw [←(nom_nom_subst_symm ji f3)]
           exact ax_q2_nom (φ[x//i]) v j
     | @ax_name    v        =>
-        simp only [nom_subst_svar]
         exact ax_name v
     | @ax_nom   φ v m n    =>  
         simp only [nom_subst_svar, nec_subst_nom, pos_subst_nom]
-        exact @ax_nom (φ[x//i]) v m n
+        apply ax_nom
     | @ax_brcn  φ v        =>
-        simp only [nom_subst_svar]
-        exact @ax_brcn (φ[x//i]) v
+        apply ax_brcn
 
-  lemma dbl_subst_nom {j : NOM} {x : SVAR} (i : NOM) (h : nom_occurs j φ = false) : φ[j//i][x//j] = φ[x//i] := by
-    induction φ <;> simp [nom_occurs, nom_subst_nom, nom_subst_svar, -implication_disjunction, *] at *
-    . split <;> simp [nom_subst_svar, Ne.symm h]
-    repeat simp [h, *] at *
-
-  lemma svar_svar_nom_subst {i j : NOM} {x : SVAR} (h : x ≥ φ.new_var) : φ[x//i][j//x] = φ[j//i] := by
-    induction φ <;> simp [nom_subst_svar, nom_subst_nom, subst_nom, -implication_disjunction, *] at *
-    . apply Ne.symm; apply diffsvar; assumption
-    . split <;> simp [subst_nom]
-    . simp [new_var_geq1 h, *] at *
-    . simp [Form.new_var] at h
-      simp [h, *] at *
-    . split
-      . exfalso
-        have := Ne.symm (diffsvar (new_var_geq2 h).left)
-        contradiction
-      . simp [new_var_geq2 h, *] at *
-  
-  lemma nom_subst_self {i : NOM} : φ[i // i] = φ := by
-    induction φ <;> simp [nom_subst_nom, -implication_disjunction, *] at * 
-    . intro h ; apply Eq.symm; assumption
-
-  lemma eq_new_var {i j : NOM} : φ.new_var = (φ[i // j]).new_var := by
-    induction φ <;> simp [Form.new_var, nom_subst_nom, *] at * 
-    . split <;> simp [Form.new_var]
-
-  lemma generalize_constants_rev {φ : Form} {x : SVAR} (i : NOM) (h : x ≥ φ.new_var) : ⊢ (all x, φ[x // i]) → ⊢ φ := by
+  lemma generalize_constants_rev {φ : Form N} {x : SVAR} (i : NOM N) (h : x ≥ φ.new_var) : ⊢ (all x, φ[x // i]) → ⊢ φ := by
     intro pf
     have l1 := ax_q2_nom (φ[x//i]) x i
     have l2 := mp l1 pf
-    rw [@svar_svar_nom_subst φ i i x h, nom_subst_self] at l2
+    rw [svar_svar_nom_subst h, nom_subst_self] at l2
     exact l2
 
-  theorem generalize_constants_iff {φ : Form} {x : SVAR} (i : NOM) (h : x ≥ φ.new_var) : ⊢ φ ↔ ⊢ (all x, φ[x // i]) := by
-    apply Iff.intro
+  theorem generalize_constants_iff {φ : Form N} {x : SVAR} (i : NOM N) (h : x ≥ φ.new_var) : ⊢ φ iff ⊢ (all x, φ[x // i]) := by
+    apply TypeIff.intro
     . apply generalize_constants; assumption
     . apply generalize_constants_rev; assumption
 
-  theorem rename_constants (j i : NOM) (h : nom_occurs j φ = false) : ⊢ φ ↔ ⊢ (φ[j // i]) := by
-    apply Iff.intro
+  theorem pf_extended {φ : Form N} : ⊢ φ iff ⊢ φ.total := by
+    apply TypeIff.intro
+    . intro pf
+      induction pf with
+      | tautology =>
+          apply Proof.tautology
+          admit
+      | ax_k =>
+          apply Proof.ax_k
+      | ax_q1 =>
+          apply Proof.ax_q1
+          admit
+      | ax_q2_svar =>
+          admit
+      | ax_q2_nom =>
+          admit
+      | ax_name =>
+          apply Proof.ax_name
+      | ax_nom  =>
+          admit
+      | ax_brcn =>
+          apply Proof.ax_brcn
+      | mp   =>
+          apply Proof.mp
+          repeat assumption
+      | general =>
+          apply Proof.general
+          assumption
+      | necess  =>
+          apply Proof.necess
+          assumption
+    . intro pf
+      generalize hc : φ.total = φ_t at *
+      induction pf with
+      | tautology =>
+          apply Proof.tautology
+          admit
+      | @ax_k ψ_t χ_t =>
+          rw [(total_ax_k hc).choose_spec.choose_spec]
+          apply ax_k
+      | ax_q1 =>
+          admit
+      | ax_q2_svar =>
+          admit
+      | ax_q2_nom =>
+          admit
+      | ax_name =>
+          admit
+      | ax_nom  =>
+          admit
+      | ax_brcn =>
+          admit
+      | mp   =>
+          admit
+      | general =>
+          admit
+      | necess  =>
+          admit
+
+  theorem rename_constants (j i : NOM N) (h : nom_occurs j φ = false) : ⊢ φ iff ⊢ (φ[j // i]) := by
+    apply TypeIff.intro
     . intro pf
       let x := φ.new_var
       have x_geq : x ≥ φ.new_var := by simp; apply Nat.le_refl
@@ -424,16 +448,16 @@ theorem generalize_constants {φ : Form} {x : SVAR} (i : NOM) (h : x ≥ φ.new_
       rw [this] at l3
       exact l3
 
-  theorem proof_sketch (h : nocc_bulk_property l₁ l₂ φ) : ⊢ φ ↔ ⊢ (φ.bulk_subst l₁ l₂) := by
+  theorem proof_sketch (h : nocc_bulk_property l₁ l₂ φ) : ⊢ φ iff ⊢ (φ.bulk_subst l₁ l₂) := by
     induction l₁ generalizing φ l₂ with
-    | nil => cases l₂ <;> simp [Form.bulk_subst]
+    | nil => cases l₂ <;> (simp [Form.bulk_subst]; apply TypeIff.refl)
     | cons h_new t_new ih =>
         cases l₂ with
-        | nil => simp [Form.bulk_subst]
+        | nil => simp [Form.bulk_subst]; apply TypeIff.refl
         | cons h_old t_old =>
             simp [Form.bulk_subst]
             have : nom_occurs h_new φ = false := by
-                apply @nocc_bulk h_new [] []
+                apply @nocc_bulk TotalSet h_new [] []
                 simp
                 unfold nocc_bulk_property at h
                 let n: Fin (List.length (h_new :: t_new)) := ⟨0, by simp⟩ 
@@ -443,41 +467,42 @@ theorem generalize_constants {φ : Form} {x : SVAR} (i : NOM) (h : x ≥ φ.new_
                 simp
                 assumption
             have := rename_constants h_new h_old this
-            rw [this]
+            apply this.trans
             apply ih
             apply nocc_bulk_property_induction
             assumption
 
-  theorem pf_odd_noms : ⊢ φ ↔ ⊢ φ.odd_noms := by
+  theorem pf_odd_noms : ⊢ φ iff ⊢ φ.odd_noms := by
     apply proof_sketch
     apply has_nocc_bulk_property
 
-  theorem pf_odd_noms_set : Γ ⊢ φ ↔ Γ.odd_noms ⊢ φ.odd_noms := by
+  theorem pf_odd_noms_set : Γ ⊢ φ iff Γ.odd_noms ⊢ φ.odd_noms := by
     simp [SyntacticConsequence]
-    conv => lhs; rhs; intro L; rw [pf_odd_noms, odd_impl]
-    apply Iff.intro
-    . intro ⟨L, h⟩ 
-      have ⟨L', eq⟩ := odd_conj Γ L
-      rw [eq] at h 
-      exists L'
+    apply TypeIff.intro
+    . intro ⟨L, h⟩
+      have h := (odd_conj Γ L) ▸ odd_impl ▸ pf_odd_noms.mp h
+      exists L.to_odd
     . intro ⟨L', h'⟩
-      have ⟨L, eq⟩ := odd_conj_rev Γ L'
-      rw [←eq] at h'
-      exists L
+      have h' := pf_odd_noms.mpr (odd_impl.symm ▸ (odd_conj_rev Γ L').symm ▸ h')
+      exists L'.odd_to
   
-  theorem odd_noms_set_cons (Γ : Set Form) : Γ.consistent ↔ Γ.odd_noms.consistent := by
-    unfold Set.consistent
+  theorem odd_noms_set_cons (Γ : Set (Form TotalSet)) : consistent Γ ↔ consistent Γ.odd_noms := by
+    unfold consistent
     have : Form.bttm = Form.bttm.odd_noms := by simp [Form.odd_noms, Form.odd_list_noms, Form.bulk_subst]
     conv => rhs; rw [this]
-    apply not_congr
-    apply pf_odd_noms_set
+    apply Iff.intro <;> (
+      intro h1 h2
+      apply h1
+      first | apply pf_odd_noms_set.mp | apply pf_odd_noms_set.mpr
+      assumption
+    )
 
 end Nominals
 
-theorem ax_nom_instance (i : NOM) (m n : ℕ) : ⊢ (iterate_pos m (i ⋀ φ) ⟶ iterate_nec n (i ⟶ φ)) := by
+theorem ax_nom_instance {φ : Form N} (i : NOM N) (m n : ℕ) : ⊢ (iterate_pos m (i ⋀ φ) ⟶ iterate_nec n (i ⟶ φ)) := by
   let x := φ.new_var
   have x_geq : x ≥ φ.new_var := by simp [SVAR.le]
-  have l1 := @ax_nom (φ[x//i]) x m n
+  have l1 := @ax_nom N (φ[x//i]) x m n
   have l2 := ax_q2_nom (iterate_pos m (x⋀(φ[x//i]))⟶iterate_nec n (x⟶(φ[x//i]))) x i
   have l3 := mp l2 l1
   clear l1 l2
@@ -502,8 +527,8 @@ theorem ax_q2_svar_instance : ⊢ ((all x, φ) ⟶ φ) := by
 theorem Γ_univ_elim (h : Γ ⊢ (all x, φ)) : Γ ⊢ φ := by
   exact Γ_mp (Γ_theorem ax_q2_svar_instance Γ) h
 
-theorem rename_var (h1 : occurs y φ = false) (h2 : is_substable φ y x) : ⊢ φ ↔ ⊢ (φ[y // x]) := by
-  apply Iff.intro
+theorem rename_var (h1 : occurs y φ = false) (h2 : is_substable φ y x) : ⊢ φ iff ⊢ (φ[y // x]) := by
+  apply TypeIff.intro
   . intro h
     apply mp
     apply ax_q2_svar_instance
@@ -529,7 +554,7 @@ theorem rename_var (h1 : occurs y φ = false) (h2 : is_substable φ y x) : ⊢ �
     . apply general
       assumption
 
-theorem ax_q2_contrap {i : NOM} {x : SVAR} : ⊢ (φ[i//x] ⟶ ex x, φ) := by
+theorem ax_q2_contrap {i : NOM N} {x : SVAR} : ⊢ (φ[i//x] ⟶ ex x, φ) := by
   rw [Form.bind_dual]
   apply hs
   . apply tautology
@@ -558,19 +583,20 @@ theorem ax_nom_instance' (x : SVAR) (m n : ℕ) : ⊢ (iterate_pos m (x ⋀ φ) 
   apply ax_nom
 
 -- Lemma 3.6.1
-lemma b361 : ⊢ ((φ ⟶ ex x, ψ) ⟶ ex x, (φ ⟶ ψ)) := by
+lemma b361 {φ : Form N} : ⊢ ((φ ⟶ ex x, ψ) ⟶ ex x, (φ ⟶ ψ)) := by
   apply mp
   . apply tautology
     apply contrapositive'
-  . simp only [←Γ_empty, Deduction, Set.union_singleton, insert_emptyc_eq]
-    let Γ : Set Form := {∼(ex x, φ⟶ψ)}
+  . apply Γ_empty.mp; apply Deduction.mpr
+    simp only [Set.union_singleton, insert_emptyc_eq]
+    let Γ : Set (Form N) := {∼(ex x, φ⟶ψ)}
     have l1 : Γ ⊢ (∼(ex x, φ⟶ψ)) := by apply Γ_premise; simp
     rw [Form.bind_dual] at l1
-    have l2 := Γ_theorem (tautology (@dne (all x, ∼(φ⟶ψ)))) Γ
+    have l2 := Γ_theorem (tautology (@dne N (all x, ∼(φ⟶ψ)))) Γ
     have l3 := Γ_mp l2 l1
-    have l4 := Γ_theorem (@ax_q2_svar_instance x (∼(φ⟶ψ))) Γ
+    have l4 := Γ_theorem (@ax_q2_svar_instance x N (∼(φ⟶ψ))) Γ
     have l5 := Γ_mp l4 l3
-    have l6 := Γ_theorem (tautology (taut_iff_mp (@imp_neg φ ψ))) Γ 
+    have l6 := Γ_theorem (tautology (taut_iff_mp (@imp_neg N φ ψ))) Γ 
     have l7 := Γ_mp l6 l5
     have l8 := Γ_conj_elim_l l7
     have l9 := Γ_conj_elim_r l7
@@ -581,66 +607,66 @@ lemma b361 : ⊢ ((φ ⟶ ex x, ψ) ⟶ ex x, (φ ⟶ ψ)) := by
       . simp [is_free, -implication_disjunction]
       . exact l9
     have l11 := Γ_conj_intro l8 l10
-    have l12 := Γ_mp (Γ_theorem (tautology (taut_iff_mpr (@imp_neg φ (ex x, ψ)))) Γ) l11
+    have l12 := Γ_mp (Γ_theorem (tautology (taut_iff_mpr (@imp_neg N φ (ex x, ψ)))) Γ) l11
     exact l12
 
 -- Lemma 3.6.2
-lemma b362 (h : is_free x φ = false) : ⊢ ((φ ⋀ ex x, ψ) ⟶ ex x, (φ ⋀ ψ)) := by
+lemma b362 {φ : Form N} (h : is_free x φ = false) : ⊢ ((φ ⋀ ex x, ψ) ⟶ ex x, (φ ⋀ ψ)) := by
   rw [Form.bind_dual, Form.bind_dual]
   apply mp
   . apply tautology
     apply contrapositive'
-  . simp only [←Γ_empty, Deduction, Set.union_singleton, insert_emptyc_eq]
-    let Γ : Set Form :=  {∼∼(all x, ∼(φ⋀ψ))}
+  . apply Γ_empty.mp; apply Deduction.mpr
+    simp only [Set.union_singleton, insert_emptyc_eq]
+    let Γ : Set (Form N) :=  {∼∼(all x, ∼(φ⋀ψ))}
     have l1 : Γ ⊢ (all x, ∼(φ⋀ψ)) := by
       apply Γ_mp; apply Γ_theorem; apply tautology; apply dne
       apply Γ_premise; simp
-    have l2 := Γ_theorem (@ax_q2_svar_instance x (∼(φ⋀ψ))) Γ
+    have l2 := Γ_theorem (@ax_q2_svar_instance x N (∼(φ⋀ψ))) Γ
     have l3 := Γ_mp l2 l1
-    have l4 := Γ_mp (Γ_theorem (tautology (taut_iff_mpr (@neg_conj φ ψ))) Γ) l3
+    have l4 := Γ_mp (Γ_theorem (tautology (taut_iff_mpr (@neg_conj N φ ψ))) Γ) l3
     have l5 : Γ⊢ (all x, (φ⟶∼ψ)) := by
       apply Γ_univ_intro'
       simp [is_free, -implication_disjunction]
       exact l4
-    have l6 := Γ_mp (Γ_theorem (ax_q1 φ (∼ψ) h) Γ) l5
-    rw [Deduction] at l6
-    have l7 := Γ_mp (Γ_theorem (tautology (@dni (all x, ∼ψ))) (Γ ∪ {φ})) l6
-    rw [←Deduction] at l7
-    have l8 := Γ_mp (Γ_theorem (tautology (taut_iff_mp (@neg_conj φ (∼(all x, ∼ψ))))) Γ) l7
+    have l6 := Deduction.mp (Γ_mp (Γ_theorem (ax_q1 φ (∼ψ) h) Γ) l5)
+    have l7 := Deduction.mpr (Γ_mp (Γ_theorem (tautology (@dni N (all x, ∼ψ))) (Γ ∪ {φ})) l6)
+    have l8 := Γ_mp (Γ_theorem (tautology (taut_iff_mp (@neg_conj N φ (∼(all x, ∼ψ))))) Γ) l7
     exact l8
 
-lemma ex_conj_comm : ⊢ ((ex x, (φ ⋀ ψ)) ⟶ (ex x, (ψ ⋀ φ))) := by
+lemma ex_conj_comm {φ : Form N} : ⊢ ((ex x, (φ ⋀ ψ)) ⟶ (ex x, (ψ ⋀ φ))) := by
   rw [Form.bind_dual, Form.bind_dual]
   apply mp
   . apply tautology
     apply contrapositive'
-  . let Γ : Set Form := ∅ ∪ {∼∼(all x, ∼(ψ⋀φ))}
+  . apply Γ_empty.mp; apply Deduction.mpr
+    simp only [Set.union_singleton, insert_emptyc_eq]
+    let Γ : Set (Form N) := {∼∼(all x, ∼(ψ⋀φ))}
     have l1 : Γ ⊢ (∼∼(all x, ∼(ψ⋀φ))) := by apply Γ_premise; simp
-    have l2 := Γ_theorem (tautology (@dne (all x, ∼(ψ⋀φ)))) Γ
+    have l2 := Γ_theorem (tautology (@dne N (all x, ∼(ψ⋀φ)))) Γ
     have l3 := Γ_mp l2 l1
-    have l4 := Γ_theorem (@ax_q2_svar_instance x (∼(ψ⋀φ))) Γ
+    have l4 := Γ_theorem (@ax_q2_svar_instance x N (∼(ψ⋀φ))) Γ
     have l5 := Γ_mp l4 l3
-    have l6 := Γ_theorem (tautology (@conj_comm_t' ψ φ)) Γ
+    have l6 := Γ_theorem (tautology (@conj_comm_t' N ψ φ)) Γ
     have l7 := Γ_mp l6 l5
     have l8 : Γ⊢(all x, ∼(φ⋀ψ)) := by
       apply Γ_univ_intro'
       simp [is_free, -implication_disjunction]
       exact l7
-    have l9 := Γ_theorem (tautology (@dni (all x, ∼(φ⋀ψ)))) Γ
+    have l9 := Γ_theorem (tautology (@dni N (all x, ∼(φ⋀ψ)))) Γ
     have l10 := Γ_mp l9 l8
-    rw [←Γ_empty, Deduction]
     exact l10
 
-lemma b362' (h : is_free x φ = false) : ⊢ (((ex x, ψ) ⋀ φ) ⟶ ex x, (ψ ⋀ φ)) := by
-  have l1 := tautology (@conj_comm_t (ex x, ψ) φ)
-  have l2 := @b362 x φ ψ h
+lemma b362' {φ : Form N} (h : is_free x φ = false) : ⊢ (((ex x, ψ) ⋀ φ) ⟶ ex x, (ψ ⋀ φ)) := by
+  have l1 := tautology (@conj_comm_t N (ex x, ψ) φ)
+  have l2 := @b362 N x ψ φ h
   have l3 := hs l2 ex_conj_comm
   have l4 := hs l1 l3
   exact l4
 
 -- Lemma 3.6.3
-lemma b363 : ⊢ ((all x, (φ ⟶ ψ)) ⟶ ((all x, φ) ⟶ (all x, ψ))) := by
-  let Γ : Set Form := ∅ ∪ {all x, φ⟶ψ} ∪ {all x, φ}
+lemma b363  {φ : Form N} : ⊢ ((all x, (φ ⟶ ψ)) ⟶ ((all x, φ) ⟶ (all x, ψ))) := by
+  let Γ : Set (Form N) := ∅ ∪ {all x, φ⟶ψ} ∪ {all x, φ}
   have l1 : Γ ⊢ (all x, (φ ⟶ ψ)) := by apply Γ_premise; simp
   have l2 : Γ⊢(φ⟶ψ) := by
     apply Γ_mp
@@ -655,16 +681,16 @@ lemma b363 : ⊢ ((all x, (φ ⟶ ψ)) ⟶ ((all x, φ) ⟶ (all x, ψ))) := by
     apply ax_q2_svar_instance
     exact x
     exact l3
-  have l5 : Γ⊢ψ := by
+  have l5 : ⊢((all x, φ⟶ψ)⟶((all x, φ) ⟶ ψ)) := by
+    apply Γ_empty.mp; apply Deduction.mpr; apply Deduction.mpr
     apply Γ_mp
     repeat assumption
-  rw [←Deduction, ←Deduction, Γ_empty] at l5
   have l6 := general x l5
   have : is_free x (all x, φ⟶ψ) = false := by simp [is_free]
-  have l7 := @ax_q1 (all x, φ⟶ψ) ((all x, φ)⟶ψ) x this
+  have l7 := @ax_q1 N (all x, φ⟶ψ) ((all x, φ)⟶ψ) x this
   have l8 := mp l7 l6
   have : is_free x (all x, φ) = false := by simp [is_free]
-  have l9 := @ax_q1 (all x, φ) ψ x this
+  have l9 := @ax_q1 N (all x, φ) ψ x this
   have l10 := hs l8 l9
   exact l10
 
@@ -737,109 +763,102 @@ lemma nec_dual : ⊢((□ ψ)⟷∼(◇ ∼ψ)) := by
         apply dn_nec
 
 lemma diw_impl (h : ⊢(φ ⟶ ψ)) : ⊢ (◇φ ⟶ ◇ψ) := by
-  have l1 := mp (tautology (@contrapositive φ ψ)) h
+  have l1 := mp (tautology contrapositive) h
   have l2 := necess l1
-  have l3 := @ax_k (∼ψ) (∼φ)
-  have l4 := mp l3 l2
-  have l5 := mp (tautology (@contrapositive (□∼ψ) (□∼φ))) l4
-  exact l5
+  have l3 := mp ax_k l2
+  have l4 := mp (tautology contrapositive) l3
+  exact l4
 
-lemma ax_brcn_contrap : ⊢ ((◇ ex x, φ) ⟶ (ex x, ◇ φ)) := by
+lemma ax_brcn_contrap {φ : Form N} : ⊢ ((◇ ex x, φ) ⟶ (ex x, ◇ φ)) := by
   simp only [Form.diamond, Form.bind_dual]
   apply mp
   . apply tautology
-    apply @contrapositive (all x, ∼∼(□∼φ)) (□ ∼∼(all x, ∼φ))
-  . let Γ : Set Form := ∅ ∪ {all x, ∼∼(□∼φ)}
+    apply contrapositive
+  . apply Γ_empty.mp; apply Deduction.mpr
+    simp only [Set.union_singleton, insert_emptyc_eq]
+    let Γ : Set (Form N) := {all x, ∼∼(□∼φ)}
     have l1 : Γ ⊢ (all x, ∼∼(□∼φ)) := by apply Γ_premise; simp 
-    have l2 := Γ_theorem (mp (tautology iff_elim_r) (@dn_all x (□∼φ))) Γ 
+    have l2 := Γ_theorem (mp (tautology iff_elim_r) (@dn_all x N (□∼φ))) Γ 
     have l3 := Γ_mp l2 l1
-    have l4 := Γ_theorem (@ax_brcn (∼φ) x) Γ
+    have l4 := Γ_theorem (@ax_brcn N (∼φ) x) Γ
     have l5 := Γ_mp l4 l3
-    have l6 := Γ_theorem (mp (tautology iff_elim_l) (@dn_nec (all x, ∼φ))) Γ
+    have l6 := Γ_theorem (mp (tautology iff_elim_l) (@dn_nec N (all x, ∼φ))) Γ
     have l7 := Γ_mp l6 l5
-    rw [←Γ_empty, Deduction]
     exact l7
 
 section MCS
 
-theorem MCS_pf (h : Set.MCS Γ) : Γ ⊢ φ → φ ∈ Γ := by
+theorem MCS_pf (h : MCS Γ) : Γ ⊢ φ → φ ∈ Γ := by
   intro pf
   rw [←(@not_not (φ ∈ Γ))]
   intro habs
   have ⟨cons, pf_bot⟩ := h
-  have pf_bot := pf_bot habs
+  have ⟨pf_bot, _⟩ := not_forall.mp (pf_bot habs)
   clear h
-  unfold Set.consistent at cons
   apply cons
   apply Γ_mp
-  rw [←Deduction] at pf_bot
+  apply Deduction.mpr
   assumption
   assumption
 
-theorem MCS_pf_iff (h : Set.MCS Γ) : Γ ⊢ φ ↔ φ ∈ Γ := by
-  apply Iff.intro
-  . exact MCS_pf h
-  . intro
-    apply Γ_premise
-    assumption
-
-theorem MCS_thm (h : Set.MCS Γ) : ⊢ φ → φ ∈ Γ := by
+theorem MCS_thm (h : MCS Γ) : ⊢ φ → φ ∈ Γ := by
   intro
   apply MCS_pf h
   apply Γ_theorem
   assumption
 
-theorem MCS_mp (h : Set.MCS Γ) (h1 : φ ⟶ ψ ∈ Γ) (h2 : φ ∈ Γ) : ψ ∈ Γ := by
+theorem MCS_mp (h : MCS Γ) (h1 : φ ⟶ ψ ∈ Γ) (h2 : φ ∈ Γ) : ψ ∈ Γ := by
   rw [←@not_not (ψ ∈ Γ)]
   intro habs
+  have ⟨pf_bot, _⟩ := not_forall.mp (h.right habs)
   apply h.left
-  have := h.right habs
-  rw [←Deduction] at this
   apply Γ_mp
+  apply Deduction.mpr
   assumption
   apply Γ_mp
   repeat (apply Γ_premise; assumption)
 
-theorem MCS_conj (hmcs : Set.MCS Γ) (φ ψ : Form) : (φ ∈ Γ ∧ ψ ∈ Γ) ↔ (φ ⋀ ψ) ∈ Γ := by
-  rw [←MCS_pf_iff hmcs, ←MCS_pf_iff hmcs, ←MCS_pf_iff hmcs]
+theorem MCS_conj {Γ : Set (Form N)} (hmcs : MCS Γ) (φ ψ : Form N) : (φ ∈ Γ ∧ ψ ∈ Γ) ↔ (φ ⋀ ψ) ∈ Γ := by
   apply Iff.intro
-  . intro ⟨l, r⟩  
-    exact Γ_conj_intro l r
+  . intro ⟨l, r⟩
+    apply MCS_pf hmcs
+    exact Γ_conj_intro (Γ_premise l) (Γ_premise r)
   . intro h
-    exact ⟨Γ_conj_elim_l h, Γ_conj_elim_r h⟩
+    apply And.intro <;> apply MCS_pf hmcs
+    exact Γ_conj_elim_l (Γ_premise h)
+    exact Γ_conj_elim_r (Γ_premise h)
 
-theorem MCS_max {Γ : Set Form} (hmcs : Γ.MCS) : (φ ∉ Γ ↔ (∼φ) ∈ Γ) := by
+theorem MCS_max {Γ : Set (Form N)} (hmcs : MCS Γ) : (φ ∉ Γ ↔ (∼φ) ∈ Γ) := by
   apply Iff.intro
   . intro h
-    rw [←MCS_pf_iff hmcs, Form.neg, Deduction]
-    exact hmcs.2 h
-  . rw [←MCS_pf_iff hmcs, ←MCS_pf_iff hmcs]
-    intro h habs
+    have ⟨pf_bot, _⟩ := not_forall.mp (hmcs.2 h)
+    apply MCS_pf hmcs; apply Deduction.mpr
+    exact pf_bot
+  . intro h habs
     apply hmcs.1
-    apply Γ_mp h habs
+    apply Γ_mp (Γ_premise h) (Γ_premise habs)
 
-theorem MCS_impl {Γ : Set Form} (hmcs : Γ.MCS) : (φ ∈ Γ → ψ ∈ Γ) ↔ ((φ⟶ψ) ∈ Γ) := by
+theorem MCS_impl {Γ : Set (Form N)} (hmcs : MCS Γ) : (φ ∈ Γ → ψ ∈ Γ) ↔ ((φ⟶ψ) ∈ Γ) := by
   apply Iff.intro
   . intro h
     by_cases hc : φ ∈ Γ
-    . simp only [←MCS_pf_iff, hmcs] at hc h ⊢
-      rw [Deduction]
+    . apply MCS_pf hmcs
+      apply Deduction.mpr
       apply increasing_consequence
-      exact h hc
+      exact Γ_premise (h hc)
       simp
     . simp only [MCS_max, hmcs, Form.neg] at hc
-      simp only [←MCS_pf_iff, hmcs, Deduction] at hc ⊢
+      apply MCS_pf hmcs; apply Deduction.mpr
       apply Γ_mp
-      apply @Γ_theorem (⊥ ⟶ ψ)
+      apply @Γ_theorem N (⊥ ⟶ ψ)
       apply tautology
       eval
-      exact hc
-  . simp only [←MCS_pf_iff, hmcs]
-    intro h1 h2
-    apply Γ_mp
-    repeat assumption
+      exact Deduction.mp (Γ_premise hc)
+  . intro h1 h2
+    apply MCS_pf hmcs
+    exact Γ_mp (Γ_premise h1) (Γ_premise h2)
 
-theorem MCS_iff {Γ : Set Form} (hmcs : Γ.MCS) : ((φ⟷ψ) ∈ Γ) ↔ (φ ∈ Γ ↔ ψ ∈ Γ) := by
+theorem MCS_iff {Γ : Set (Form N)} (hmcs : MCS Γ) : ((φ⟷ψ) ∈ Γ) ↔ (φ ∈ Γ ↔ ψ ∈ Γ) := by
   simp only [Form.iff, ←MCS_conj, ←MCS_impl, hmcs]
   apply Iff.intro
   <;> intros; apply Iff.intro
@@ -849,18 +868,19 @@ theorem MCS_iff {Γ : Set Form} (hmcs : Γ.MCS) : ((φ⟷ψ) ∈ Γ) ↔ (φ ∈
     assumption
   apply And.intro <;> simp [*]
 
-theorem MCS_rw {Γ : Set Form} (hmcs : Γ.MCS) (pf : ⊢ (φ ⟷ ψ)) : φ ∈ Γ ↔ ψ ∈ Γ := by
-  rw [←MCS_iff hmcs, ←MCS_pf_iff hmcs]
+theorem MCS_rw {Γ : Set (Form N)} (hmcs : MCS Γ) (pf : ⊢ (φ ⟷ ψ)) : φ ∈ Γ ↔ ψ ∈ Γ := by
+  rw [←MCS_iff hmcs]
+  apply MCS_pf hmcs
   exact Γ_theorem pf Γ
 
-lemma MCS_rich : ∀ {Θ : Set Form}, (Θ.MCS) → (Θ.witnessed) → ∃ i : NOM, ↑i ∈ Θ := by
+lemma MCS_rich : ∀ {Θ : Set (Form N)}, (MCS Θ) → (witnessed Θ) → ∃ i : NOM N, ↑i ∈ Θ := by
   intro Θ mcs wit
   have := Proof.MCS_thm mcs (Proof.ax_name ⟨0⟩)
   have := wit this
   simp [subst_nom] at this
   exact this
 
-lemma MCS_with_svar_witness : ∀ {Θ : Set Form} {x y : SVAR} (_ : is_substable φ y x), (Θ.MCS) → φ[y//x] ∈ Θ → (ex x, φ) ∈ Θ := by
+lemma MCS_with_svar_witness : ∀ {Θ : Set (Form N)} {x y : SVAR} (_ : is_substable φ y x), (MCS Θ) → φ[y//x] ∈ Θ → (ex x, φ) ∈ Θ := by
   intro Θ x y h1 mcs h2
   apply MCS_mp mcs
   apply MCS_thm mcs
